Environment.v
@@ -1,0 +1,160 @@
+Require Import Velus.Common.
+
+Require Import List.
+Require Import Coq.Structures.OrderedType.
+Require Import Coq.Structures.OrderedTypeEx.
+
+Module POTB := PositiveOrderedTypeBits.
+
+Import List.ListNotations.
+
+Set Implicit Arguments.
+
+Definition t (A: Type) := list (ident * A).
+
+Section Global.
+
+  Variable A B: Type.
+
+  Fixpoint find (x: ident) (e: t A) : option A :=
+    match e with
+    | [] => None
+    | (y, a) :: e' =>
+      match POTB.compare x y with
+      | LT _ => None
+      | EQ _ => Some a
+      | GT _ => find x e'
+      end
+    end.
+
+  Fixpoint add (x: ident) (a: A) (e: t A) : t A :=
+    match e with
+    | [] => [(x, a)]
+    | (y, b) :: e' =>
+      match POTB.compare x y with
+      | LT _ => (x, a) :: e
+      | EQ _ => (x, a) :: e'
+      | GT _ => (y, b) :: add x a e'
+      end
+    end.
+
+  Definition map (f: A -> B) (e: t A) : t B :=
+    List.map (fun (xa: ident * A) =>
+                let (x, a) := xa in
+                (x, f a))
+             e.
+
+  Definition mapi (f: ident -> A -> B) (e: t A) : t B :=
+    List.map (fun (xa: ident * A) =>
+                let (x, a) := xa in
+                (x, f x a))
+             e.
+
+  Fact compare_eq:
+    forall x,
+    exists H, POTB.compare x x = EQ H.
+  Proof.
+    intros; destruct (POTB.compare x x) as [|Eq|];
+      try (now exfalso; eapply POTB.bits_lt_antirefl; eauto).
+    exists Eq; auto.
+  Qed.
+
+  Theorem gss:
+    forall x a e,
+      find x (add x a e) = Some a.
+  Proof.
+    induction e as [|[y]]; simpl.
+    - destruct (compare_eq x) as [? E]; now rewrite E.
+    - destruct (POTB.compare x y) eqn: Cmp; simpl.
+      + destruct (compare_eq x) as [? E]; now rewrite E.
+      + destruct (compare_eq x) as [? E]; now rewrite E.
+      + now rewrite Cmp.
+  Qed.
+
+  Corollary gss':
+    forall x y a e,
+      ident_eqb x y = true ->
+      find x (add y a e) = Some a.
+  Proof.
+    intros ** E; rewrite ident_eqb_eq in E; subst; apply gss.
+  Qed.
+
+  Theorem gso:
+    forall x y a e,
+      x <> y ->
+      find x (add y a e) = find x e.
+  Proof.
+    induction e as [|[z]]; intros Neq; simpl.
+    - destruct (POTB.compare x y); simpl; auto.
+      now contradict Neq.
+    - destruct (POTB.compare y z) eqn: Eyz, (POTB.compare x z) eqn: Exz, (POTB.compare x y) eqn: Exy;
+        simpl; try rewrite Exy; try rewrite Exz; auto;
+          try (now contradict Neq);
+          try repeat match goal with
+                H: POTB.eq ?a ?b |- _ =>
+                assert (a = b); auto; subst b;
+                  exfalso; apply (POTB.bits_lt_antirefl a);
+                    etransitivity; eauto
+              end.
+      exfalso; apply (POTB.bits_lt_antirefl x);
+        do 2 (etransitivity; eauto).
+  Qed.
+
+  Corollary gso':
+    forall x y a e,
+      ident_eqb x y = false ->
+      find x (add y a e) = find x e.
+  Proof.
+    intros ** E; rewrite ident_eqb_neq in E; now apply gso.
+  Qed.
+
+  Lemma find_cons_eq:
+    forall x a e,
+      find x ((x, a) :: e) = Some a.
+  Proof.
+    intros; simpl.
+    destruct (compare_eq x) as [? E]; now rewrite E.
+  Qed.
+
+  Lemma find_cons_lt:
+    forall x y a e,
+      POTB.lt x y ->
+      find x ((y, a) :: e) = None.
+  Proof.
+    intros ** E; simpl.
+    destruct (POTB.compare x y) eqn: Exy; auto.
+    - assert (x = y); auto; subst; contradict E; apply POTB.bits_lt_antirefl.
+    - exfalso; apply (POTB.bits_lt_antirefl x);
+        do 2 (etransitivity; eauto).
+  Qed.
+
+  Theorem find_in:
+    forall x a e,
+      find x e = Some a ->
+      In (x, a) e.
+  Proof.
+    induction e as [|(y, b)]; simpl.
+    - intro; discriminate.
+    - intro H; destruct (POTB.compare x y); try discriminate.
+      + assert (x = y); auto; inv H; auto.
+      + right; auto.
+  Qed.
+
+End Global.
+
+Theorem find_map:
+  forall (A B: Type) (x: ident) (e: t A) (f: A -> B),
+    find x (map f e) = option_map f (find x e).
+Proof.
+  induction e as [|[y]]; simpl; intros; auto.
+  destruct (POTB.compare x y); auto.
+Qed.
+
+Theorem find_mapi:
+  forall (A B: Type) (x: ident) (e: t A) (f: ident -> A -> B),
+    find x (mapi f e) = option_map (f x) (find x e).
+Proof.
+  induction e as [|[y]]; simpl; intros; auto.
+  destruct (POTB.compare x y); auto.
+  assert (x = y); auto; subst; auto.
+Qed.
